Top-level proof goes through.  Now the fun begins.

ironfleet/src/Dafny/Distributed/Services/Lock/TrueMain.i.dfy
@@ -5,7 +5,7 @@ module TrueMain_i {
     import opened Main_i
     import opened QuantizedSystem_s 
 
-    function LeaseSpecIoFilter(config:ConcreteConfiguration) : IoPredicate
+    function {:axiom} LeaseSpecIoFilter(config:ConcreteConfiguration) : IoPredicate
         ensures forall io :: LeaseSpecIoFilter(config).requires(io);
 //    {
 //        (io:IoOp) -> exists epoch :: io.LIoOpReceive?
@@ -155,54 +155,213 @@ module TrueMain_i {
         */
     }
 
+    lemma ProjectDsExternalIO_premium(db:seq<DS_State>, external_io:IoPredicate) returns (trace:IoTrace)
+        requires forall io :: external_io.requires(io);
+        ensures  trace == ProjectDsExternalIO(db, external_io);
+        ensures  forall projected_index :: 0 <= projected_index < |trace| ==> 
+                     (exists db_index :: 0 <= db_index < |db| && 
+                        var step := db[db_index].environment.nextStep;
+                        step.LEnvStepHostIos? && |step.ios| == 1 && external_io(step.ios[0]) &&
+                        step.ios[0] == trace[projected_index]);
+    {
+        if db == [] {
+            trace := [];
+        } else {
+            var step := db[0].environment.nextStep;
+            if step.LEnvStepHostIos? && |step.ios| == 1 && external_io(step.ios[0]) {
+                var rest := ProjectDsExternalIO_premium(db[1..], external_io);
+                trace := step.ios + rest;
+//                assert forall projected_index :: 0 <= projected_index < |trace| 
+//                        ==> exists db_index :: 0 <= db_index < |db| && 
+//                        var step := db[db_index].environment.nextStep;
+//                        step.LEnvStepHostIos? && |step.ios| == 1 && external_io(step.ios[0]) &&
+//                        step.ios[0] == trace[projected_index];
+            } else {
+                trace := ProjectDsExternalIO_premium(db[1..], external_io);
+            }
+        }
+    }
+
+
     ghost method FindProjectDsExternalIOIndex(db:seq<DS_State>, external_io:IoPredicate, projected_index:int) returns (db_index:int)
         requires forall io :: external_io.requires(io);
-        ensures  0 <= projected_index < |ProjectDsExternalIO(db, external_io)|;
+        requires 0 <= projected_index < |ProjectDsExternalIO(db, external_io)|;
         ensures  0 <= db_index < |db|;
         ensures  var step := db[db_index].environment.nextStep;
                  step.LEnvStepHostIos? && |step.ios| == 1 && external_io(step.ios[0])
         ensures  ProjectDsExternalIO(db, external_io)[projected_index] == db[db_index].environment.nextStep.ios[0];
     {
-        if qb == [] then
+        var trace := ProjectDsExternalIO_premium(db, external_io);        
+        db_index :| 0 <= db_index < |db| &&
+                    var step := db[db_index].environment.nextStep;
+                    step.LEnvStepHostIos? && |step.ios| == 1 && external_io(step.ios[0])
+                 && step.ios[0] == ProjectDsExternalIO(db, external_io)[projected_index];
 
 
     }
 
+    predicate P()
 
-    lemma UltimateRefinementProof(config:ConcreteConfiguration, qb:seq<QS_State>) returns (sb:seq<ServiceState>)
+    lemma ServiceCorrespondenceTransfers(step1:LEnvStep<EndPoint, seq<byte>>, step2:LEnvStep<EndPoint, seq<byte>>, serviceState:ServiceState)
+        requires Service_Correspondence(step1, serviceState);
+        requires step1.LEnvStepHostIos? && step2.LEnvStepHostIos?;
+        requires forall io :: io in step2.ios ==> io in step1.ios;
+        ensures  Service_Correspondence(step2, serviceState);
+    {
+
+    }
+    
+    lemma lemma_ServiceConsistency(config:ConcreteConfiguration, sb:seq<ServiceState>, i:int)
+        requires |sb| > 0 //&& Service_Init(sb[0], config) 
+              && forall j :: //{:trigger Service_Next(sb[j], sb[j+1])} :: 
+                    0 <= j < |sb| - 1 ==> sb[j] == sb[j+1] || Service_Next(sb[j], sb[j+1])
+        requires 0 <= i < |sb|;
+        ensures  sb[i].hosts == sb[0].hosts;
+        //ensures  Collections__Maps2_s.mapdomain(db[i].servers) == Collections__Maps2_s.mapdomain(db[0].servers);
+    {
+        if i == 0 {
+        } else {
+//            if sb[i] != sb[i-1] {
+//                //var j := i - 1;
+//                //assert Service_Next(sb[j], sb[j+1]);
+//            }
+            lemma_ServiceConsistency(config, sb, i - 1);
+        }
+    }
+
+
+    lemma UltimateRefinementProof(config:ConcreteConfiguration, qb:seq<QS_State>) returns (qb':seq<QS_State>, sb:seq<ServiceState>)
         requires |qb| > 0;
         requires QS_Init(qb[0], config);
         requires forall i {:trigger QS_Next(qb[i], qb[i+1])} :: 0 <= i < |qb| - 1 ==> QS_Next(qb[i], qb[i+1]);
+        requires exists qs_ultimate :: QS_Next(last(qb), qs_ultimate);
         requires var trace:StepTrace := ComputeStepTrace(qb);
                  forall host :: host in qb[0].servers ==> 
                      exists io_partition:seq<IoTrace>, behavior:seq<HostState> :: 
                          SeqCat(io_partition) == ProjectStepTraceToHostIos(trace, host) 
                       && |io_partition| == |behavior| - 1
                       && (forall i :: 0 <= i < |io_partition| ==> HostNext(behavior[i], behavior[i+1], io_partition[i])); 
-        ensures  |qb| == |sb|;
+        ensures  |qb| == |qb'| == |sb|;
         ensures  Service_Init(sb[0], Collections__Maps2_s.mapdomain(qb[0].servers));
         ensures  forall i {:trigger Service_Next(sb[i], sb[i+1])} :: 0 <= i < |sb| - 1 ==> (sb[i] == sb[i+1]) || Service_Next(sb[i], sb[i+1]);
-        ensures  forall i :: 0 <= i < |qb| ==> Service_Correspondence(qb[i].environment.nextStep, sb[i]);
+        ensures  ProjectExternalIO(qb, LeaseSpecIoFilter(config)) == ProjectExternalIO(qb', LeaseSpecIoFilter(config)); 
+        ensures  forall i :: 0 <= i < |qb'| ==> Service_Correspondence(qb'[i].environment.nextStep, sb[i]);
     {
-        var qb', db' := BryansProof(config, qb, LeaseSpecIoFilter); 
+        var db';
+        qb', db' := BryansProof(config, qb, LeaseSpecIoFilter); 
 
         sb := RefinementProof(config, db');
 
-        forall i {:trigger Service_Correspondence(qb[i].environment.nextStep, sb[i])} | 0 <= i < |qb| 
-          ensures Service_Correspondence(qb[i].environment.nextStep, sb[i]);
+        forall qb_index {:trigger Service_Correspondence(qb'[qb_index].environment.nextStep, sb[qb_index])} 
+               | 0 <= qb_index < |qb'| 
+          ensures Service_Correspondence(qb'[qb_index].environment.nextStep, sb[qb_index]);
         {
-          assert Service_Correspondence(db'[i].environment.nextStep, sb[i]);
+          assert Service_Correspondence(db'[qb_index].environment.nextStep, sb[qb_index]);
           LeaseSpecIoFilterDefn();
 
-          var step := qb[i].environment.nextStep;
-          if step.LEnvStepHostIos? && |step.ios| == 1 && LeaseSpecIoFilter(config)(step.ios[0]) {
+          var step := qb'[qb_index].environment.nextStep;
+          var external_io := LeaseSpecIoFilter(config);
+          if step.LEnvStepHostIos? && |step.ios| == 1 && external_io(step.ios[0]) {
+              var d_step := db'[qb_index].environment.nextStep;
+              assert d_step.LEnvStepHostIos? && step.ios[0] in d_step.ios;
+              assert |step.ios| == 1;
+
+              ServiceCorrespondenceTransfers(d_step, step, sb[qb_index]);
             
-            var projected_index := FindProjectExternalIOIndex(qb, LeaseSpecIoFilter(config), i); 
-            assert Service_Correspondence(qb[i].environment.nextStep, sb[i]);
+            /*
+            var projected_index := FindProjectExternalIOIndex(qb', external_io, qb_index); 
+            var db_index := FindProjectDsExternalIOIndex(db', external_io, projected_index);
+            assert Service_Correspondence(db'[db_index].environment.nextStep, sb[db_index]);
+
+            calc {
+                qb'[qb_index].environment.nextStep.ios[0];
+                ProjectExternalIO(qb, external_io)[projected_index];
+                ProjectDsExternalIO(db', external_io)[projected_index];
+                db'[db_index].environment.nextStep.ios[0];
+            }
+            assert |qb'[qb_index].environment.nextStep.ios| == 1;
+
+            var serviceState := sb[qb_index];
+
+            assert db_index == qb_index;
+            */
+
+//            ServiceCorrespondenceTransfers(db'[db_index].environment.nextStep, step, sb[db_index]);
+//            forall io, epoch | 
+//                    step.LEnvStepHostIos? 
+//                 && io in step.ios
+//                 && io.LIoOpReceive?
+//                 && io.r.msg == MarshallLockMsg(epoch) 
+//                 && io.r.src in serviceState.hosts 
+//                 && io.r.dst !in serviceState.hosts
+//                ensures 1 <= epoch <= |serviceState.history| && io.r.src == serviceState.history[epoch-1];
+//            {
+//                assert io in qb[qb_index].environment.nextStep.ios;
+//                var i :| 0 <= i < |qb[qb_index].environment.nextStep.ios| && qb[qb_index].environment.nextStep.ios[i] == io;
+//                assert i == 0;
+//                assert io == qb[qb_index].environment.nextStep.ios[0];
+//                assert io in db'[db_index].environment.nextStep.ios;
+//                assert io.r.msg == MarshallLockMsg(epoch);
+//            }
+//            assume P() && !P();
+                
+            assert Service_Correspondence(qb'[qb_index].environment.nextStep, sb[qb_index]);
           } else {
-            assert Service_Correspondence(qb[i].environment.nextStep, sb[i]);
+            //assume P() && !P();
+            if !step.LEnvStepHostIos? {
+                assert Service_Correspondence(qb'[qb_index].environment.nextStep, sb[qb_index]);
+            } else if |step.ios| != 1 {
+                assert step.LEnvStepHostIos?;
+                if qb_index < |qb'| - 1 {
+                    assert QS_Next(qb'[qb_index], qb'[qb_index + 1]);
+                } else {
+                    assert qb_index == |qb'| - 1;
+                    var qs_ultimate :| QS_Next(last(qb'), qs_ultimate);
+                    assert last(qb') == qb'[qb_index];
+                }
+//                assert step == qb'[qb_index].environment.nextStep;
+//                assert |step.ios| <= 1;
+//                assert |step.ios| == 0;
+                
+                assert Service_Correspondence(qb'[qb_index].environment.nextStep, sb[qb_index]);
+            } else if !external_io(step.ios[0]) {
+                //var io := step.ios[0];
+                var serviceState := sb[qb_index];
+
+                calc {
+                    serviceState.hosts;
+                        { lemma_ServiceConsistency(config, sb, qb_index); }
+                    sb[0].hosts;
+                    Collections__Maps2_s.mapdomain(db'[0].servers);
+                    MapSeqToSet(config, x=>x);
+                }
+                forall h | h in config
+                    ensures h in serviceState.hosts;
+                { }
+                forall h | h in serviceState.hosts
+                    ensures h in config;
+                { }
+
+                //assert serviceState.hosts == config;
+                forall io, epoch | io in step.ios
+                    ensures !(   io.LIoOpReceive?
+                              && io.r.msg == MarshallLockMsg(epoch) 
+                              && io.r.src in serviceState.hosts 
+                              && io.r.dst !in serviceState.hosts);
+                {
+                    assert io == step.ios[0];
+                    assert !(   io.LIoOpReceive?
+                             && io.r.msg == MarshallLockMsg(epoch) 
+                             && io.r.src in config
+                             && io.r.dst !in config);
+                }
+
+                assert Service_Correspondence(qb'[qb_index].environment.nextStep, sb[qb_index]);
+            } else {
+                assert false;
+            }
           }
-          assert Service_Correspondence(qb[i].environment.nextStep, sb[i]);
+          assert Service_Correspondence(qb'[qb_index].environment.nextStep, sb[qb_index]);
         }
     }
 }
